bedrock2/src/bedrock2/FE310CSemantics.v
@@ -2,6 +2,7 @@ Require Import Coq.ZArith.ZArith.
 Require Import bedrock2.Syntax bedrock2.Semantics.
 Require coqutil.Datatypes.String coqutil.Map.SortedList coqutil.Map.SortedListString.
 Require Import coqutil.Word.Interface.
+Require Import coqutil.Word.Bitwidth32.
 Require coqutil.Word.Naive.
 Require Import coqutil.Z.HexNotation.
 
