compiler/src/compiler/ForeverSafe.v
@@ -17,7 +17,7 @@ Import ListNotations.
 
 Section ForeverSafe.
 
-  Context {W: Words}.
+  Context {width} {BW: Bitwidth width} {word: word.word width} {word_ok: word.ok word}.
   Context {Registers: map.map Z word}.
   Context {mem: map.map word byte}.
 
